platform/cito/SepLemmas.v
@@ -1,5 +1,10 @@
-Require Import AutoSep.
+Require Import Inv.
 
+Lemma is_heap_upd_option_bwd : forall layout h addr a, layout_option layout addr a * is_heap layout h ===> is_heap layout (heap_upd_option h addr a).
+  admit.
+Qed.
+
+(*
 Lemma star_diff_ptrs : forall specs st p1 p2, interp specs (![p1 =?>1 * p2 =?> 1] st) -> p1 <> p2.
   rewrite sepFormula_eq.
   propxFo.
@@ -31,3 +36,4 @@ Lemma star_diff_ptrs : forall specs st p1 p2, interp specs (![p1 =?>1 * p2 =?> 1
   rewrite H in H4.
   discriminate.
 Qed.
+*)
